

@prefix skos: <http://www.w3.org/2004/02/skos/core#> .
@prefix pensoft: <http://id.pensoft.net/> .
@prefix rdf: <http://www.w3.org/1999/02/22-rdf-syntax-ns#> .
@prefix foaf: <http://xmlns.com/foaf/0.1/> .
@prefix pro: <http://purl.org/spar/pro/> .
@prefix scoro: <http://purl.org/spar/scoro/> .
@prefix ti: <http://www.ontologydesignpatterns.org/cp/owl/timeinterval.owl#> .
@prefix tvc: <http://www.essepuntato.it/2012/04/tvc/> .
@prefix xsd: <http://www.w3.org/2001/XMLSchema#> .
@prefix fabio: <http://purl.org/spar/fabio/> .
@prefix dcterms: <http://purl.org/dc/terms/> .
@prefix dc: <http://purl.org/dc/elements/1.1/> .
@prefix frbr: <http://purl.org/vocab/frbr/core#> .
@prefix prism: <http://prismstandard.org/namespaces/basic/2.0/> .
@prefix doco: <http://purl.org/spar/doco/> .
@prefix po: <http://www.essepuntato.it/2008/12/pattern#> .
@prefix co: <http://purl.org/co/> .
@prefix trt: <http://plazi.org/treatment#> .
@prefix c4o: <http://purl.org/spar/c4o/> .
@prefix dwciri: <http://rs.tdwg.org/dwc/iri/> .
@prefix nomen: <http://www.semanticweb.org/dmitriev/ontologies/2013/8/untitled-ontology-6#> .
@prefix dwc: <http://rs.tdwg.org/dwc/terms/> .
@prefix sro: <http://salt.semanticauthoring.org/ontologies/sro#> .
@prefix deo: <http://purl.org/spar/deo/> .
@prefix pext: <http://proton.semanticweb.org/protonue#> .
@prefix ptop: <http://proton.semanticweb.org/protont#> .
@prefix pkm: <http://proton.semanticweb.org/protonkm#> .
@prefix : <http://openbiodiv.net/> .

: rdf:type owl:Ontology ;
  owl:versionInfo "0.3" ;
  rdfs:comment "Open Biodiversity Knowledge Management System Ontology" ;
  dc:title "OpenBiodiv Ontology" ;
  dc:subject "OpenBiodiv Ontology" ;
  rdfs:label "OpenBiodiv Ontology" ;
  dc:creator "Viktor Senderov, Terry Catapano, Kiril Simov, Lyubomir Penev" ;
  dc:rights "CCBY" .


po:contains rdf:type owl:TransitiveProperty .

:Publisher rdf:type owl:Class ;
  rdfs:label "Publisher"@en ;
  rdfs:comment "The publisher of a journal, a type of `foaf:Agent`."@en ;
  rdfs:subClassOf foaf:Agent .

trt:Treatment a owl:Class ;
  rdfs:label "Taxonomic Treatment"@en ;
  rdfs:label "Taxonomische Abhandlung"@de ;
  rdfs:label "Таксономично пояснение"@bg ;
  rdfs:comment "A taxonomic treatment, or simply a treatment, is a 
                rhetorical element of a taxonomic publication, i.e. a 
                specialized section, where taxon circumscription  
                takes place."@en ;
  rdfs:comment "Eine taxonomische Abhandlung, oder nur Abhandlung, ist 
                ein rhetorisches Element eines wissenschaftlichen 
                taxomischen Artikels, d.h. ein spezialisierter Abschnitt,
                wo die Umschreibung eines taxonomischen Konzeptes
                stattfindet."@de ;
  rdfs:comment "Таксономично пояснение или само Пояснение е риторчна част
                от таксономичната статия, където се случва описанието
                на дадена таксономична концепция."@bg ;                  
  rdfs:subClassOf deo:DiscourseElement .

trt:Nomenclature a owl:Class ;
  rdfs:subClassOf deo:DiscourseElement ,
                  [ rdf:type owl:Restriction ;
                    owl:onProperty po:isContainedBy ;
                    owl:someValuesFrom trt:Treatment ] ;
  rdfs:label "Taxonomic Nomenclature Section"@en ;
  rdfs:comment "A taxonomic nomenclature section, or simply a
nomenclature, is a rhetorical element of a taxonomic publication where
nomenclatural acts are published and nomenclatural statements are made.
Nomenclature is a subsection of Treatment."@en .

trt:NomenclatureHeading a owl:Class ;
  rdfs:subClassOf deo:DiscourseElement ,
                  [ rdf:type owl:Restriction ;
                    owl:onProperty po:isContainedBy ;
                    owl:someValuesFrom trt:Nomenclature ] ;
                  rdfs:label "Treatment Title"@en ;
  rdfs:comment "Inside the taxonomic nomenclature section, we have the treatment title."@en .

trt:NomenclatureCitationList a owl:Class ;
  rdfs:subClassOf deo:DiscourseElement ,
                  [ rdf:type owl:Restriction ;
                    owl:onProperty po:isContainedBy ;
                    owl:someValuesFrom trt:Nomenclature ] ;
                  rdfs:label "Taxonomic Nomenclature Citation List"@en ;
  rdfs:comment "Inside the taxonomic nomenclature section, we have a list
                of citations."@en .                  

:TaxonomicNameUsage rdf:type owl:Class ;
  rdfs:subClassOf  pext:Mention ;
  rdfs:comment "A taxonomic name usage is the mentioning of a
biological taxonomic name or taxon concept label in a text."@en ;
  rdfs:label "Taxonomic Name Usage"@en .

dwciri:taxonomicStatus rdf:type owl:ObjectProperty ; 
  rdfs:label "taxonomic status"@en ;
  rdfs:comment "the IRI version of the DwC term taxonmic status" .

:BiologicalName rdf:type owl:Class ;
    rdfs:label "Biological Name"@en ;
    owl:sameAs nomen:NOMEN_0000030 .

:ScientificName rdf:type owl:Class ;
    rdfs:subClassOf :BiologicalName ;
    rdfs:label "Scientific Name"@en ;
    owl:sameAs  nomen:NOMEN_0000036 .
    
:VernacularName a owl:Class ;
  rdfs:subClassOf :BiologicalName ;
  rdfs:label "Vernacular Name"@en ;
  owl:sameAs nomen:NOMEN_0000037 .

dwciri:scientificName rdf:type owl:ObjectProperty ;
  rdfs:label "scientific name"@en;
  rdfs:comment "the IRI version of dwc:scientificName"@en .

dwciri:nameAccordingTo rdf:type owl:ObjectProperty ;
  rdfs:label "name according to" ;
  rdfs:comment "the IRI version of dwc:scientificName"@en . 
  
:biologicalName rdf:type owl:ObjectProperty ;
  rdfs:subPropertyOf pkm:mentions ;
        rdfs:label "mentions biological name"@en ;
        rdfs:range :BiologicalName .

:vernacularName rdf:type owl:ObjectProperty ;
  rdfs:subPropertyOf :biologicalName ;
        rdfs:label "mentions vernacular name" @en ;
        rdfs:range :VernacularName .

:scientificName rdf:type owl:ObjectProperty ;
  rdfs:subPropertyOf dwciri:scientificName, :biologicalName ;
  rdfs:label "mentions scientific name"@en ; 
  rdfs:range :ScientificName ;
  rdfs:comment "'the scientific name property, derived from ':biologicalName', 'pkm:mentions', and 'dwciri:scientificName"@en .

:taxonConceptLabel rdf:type owl:ObjectProperty ;
  rdfs:subPropertyOf :biologicalName ;
  rdfs:label "mentions taxon concept label"@en ;
  rdfs:range :TaxonConceptLabel .

:nameAccordingTo rdf:type owl:ObjectProperty ;
  rdfs:label "sec."@en ; 
  rdfs:range frbr:Expression ;
  rdfs:comment "The reference to the source in which the specific taxon concept circumscription is defined or implied - traditionally signified by the Latin 'sensu' or 'sec.'' (from secundum, meaning 'according to'). For taxa that are relevantly circumscribed by identifications, a reference to the keys, monographs, experts and other sources should be given. Should only be used with IRI's"@en .

:relatedName rdf:type owl:ObjectProperty, owl:TransitiveProperty, owl:ReflexiveProperty ;
  rdfs:label "has related name"@en ;
  rdfs:domain :BiologicalName ;
  rdfs:range :BiologicalName ;
  rdfs:comment "'has related name' is an object property that we
use in order to indicate that two biological names are related somehow. This
relationship is purposely vague as to encompass all situations where two
biological names co-occur in a text. It is transitive and reflexive."@en.


:replacementName rdf:type owl:ObjectProperty ,
                          owl:TransitiveProperty ;
  rdfs:label "has replacement name"@en ;
  rdfs:domain :ScientificName ;
  rdfs:range :ScientificName ;
  rdfs:comment "This is a uni-directional property. Its meaning
is that one one biological name links to a different biological name via the
usage of this property, then the object of the triple is the form of the
biological name the use of which is more accurate and should be preferred
given the information that system currently holds. This property is only
defined for scientific names."@en.

:TaxonConcept rdf:type owl:Class ;
  owl:equivalentClass dwc:Taxon ;
  rdfs:subClassof frbr:Work , skos:Concept ,
                  [ rdf:type owl:Restriction ;
                    owl:onProperty :taxonConceptLabel ;
                    owl:minCardinality "1" ] .

:RCC5Statement rdf:type owl:Class ;
  rdfs:label "RCC5 Statement" ;
  rdfs:comment "A statemnt of RCC-5 relationship" .

:rcc5Property rdf:Type owl:ObjectProperty ;
  rdfs:domain :RCC5Statement .

:rcc5fromRegion rdf:type owl:ObjectProperty ;
  rdfs:subPropertyOf :rcc5Property ;
  rdfs:label "from region" ;
  rdfs:comment "Connects to the RCC5 statement to the originating region"@en .

:rcc5toRegion rdf:type owl:ObjectProperty ;
  rdfs:label "to region" ;
  rdfs:subPropertyOf :rcc5Property ;
  rdfs:comment "Connects to the RCC5 statement to the target region"@en .

:rcc5RelationType rdf:type owl:ObjectProperty ;
  rdfs:label "relation type" ;
  rdfs:subPropertyOf :rcc5Property ;
  rdfs:range :RCC5Relation ;
  rdfs:comment "Connects an RCC-5 statement to the type of RCC-5 relation between the regions."@en .

:TaxonomicStatus rdf:type owl:Class ;
  rdfs:subClassOf [ rdf:type owl:Restriction ;
                    owl:onProperty <http://www.w3.org/2004/02/skos/core#inScheme> ;
                    owl:someValuesFrom :TaxonomicStatusTerms ] ;
  rdfs:label "Taxonomic Status"@en ;
  rdfs:comment "The status following a taxonomic name usage in a taxonomic
                manuscript, i.e. 'n. sp.',
                                 'comb. new',
                                 'sec. Franz (2017)', etc"@en .

:TaxonomicStatusTerms rdf:type owl:Class ;
  rdfs:subClassOf <http://www.w3.org/2004/02/skos/core#ConceptScheme> ,
                                [ rdf:type owl:Restriction ;
                                  owl:onProperty fabio:isSchemeOf ;
                                  owl:allValuesFrom :TaxonomicStatus] ;
  rdfs:label "OpenBiodiv Vocabulary of Taxonomic Statuses"@en ;
  fabio:hasDiscipline <http://dbpedia.org/page/Taxonomy_(biology)> .

  
  :TaxonomicUncertainty a :TaxonomicStatus ;
    rdfs:label "Taxonomic Uncertainty"@en ;
    skos:inScheme :TaxonomicStatusTerms ;
    skos:related <http://rs.gbif.org/vocabulary/gbif/taxonomicStatus/accepted> ;
   
    rdfs:comment "The implication of this term that the taxon concept identified
  by a name has an uncertain placement in the biological taxonomy, or if we
  are talking about a specimen or a sample of some kind that we are unable to
  identify the taxon down to its rank. "@en .

  
  :TaxonDiscovery a :TaxonomicStatus ;
    skos:inScheme :TaxonomicStatusTerms ;
    rdfs:label "Taxon Discovery"@en ;

    rdfs:comment "When a TNU is followed by the term `:TaxonDiscovery`, the
  implication is that the present context in which the TNU is used is
  circumscribing a new taxon concept (a taxon concept of a taxon new to
  science), and simultaneously assigning it a new name."@en .

  
  :ReplacementName a :TaxonomicStatus ;
    skos:inScheme :TaxonomicStatusTerms ;
    rdfs:label "Replacement Name"@en ;
    rdfs:comment "When a TNU is followed by the term `:ReplacementName`, the implication is that
  the name that is referred to by the TNU is replacing another name for various
  reasons, and thus becoming the preferred/accepted/available way of refering to
  whatever taxon concepts the now replaced name had been referring to. Cases
  include changes of rank, new combinations, spelling mistakes, etc.
  "@en .

  
  :UnavailabeName a :TaxonomicStatus ;
    skos:inScheme :TaxonomicStatusTerms ;
    rdfs:label "UnavailableName"@en ;
    skos:exactMatch  <http://rs.gbif.org/vocabulary/gbif/taxonomicStatus/synonym> ;
    rdfs:comment "When a TNU is followed by the term `:UnavailableName`, the implication is that
  the name that is being referred to by the TNU is no longer or has never been
  available for use due to the fact that it has either been replaced or it has
  been determined that the name has been improperly coined or published, or the
  name contains any general error rendering it unfit for use."@en .
  
  :AvailableName a :TaxonomicStatus ;
    skos:inScheme :TaxonomicStatusTerms ;
    rdfs:Label "Available Name"@en ;
    skos:exactMatch <http://rs.gbif.org/vocabulary/gbif/taxonomicStatus/accepted> ;
    rdfs:comment "When a TNU is followed by the term `:AvailableName`, the
  implication is that the name that is being referred to by the TNU has been
  determined to be fit for use either by revoking an older act rendering the
  name unavailable or by fixing other issues with the name or finding out that
  other issues with the name had been fixed, or just stating the fact that the
  name shall be used or even conserving it, so that the name can be freely used
  from then on in compliance with all Codes and practices."@en.
  
  :TypeSpecimenDesignation a :TaxonomicStatus ;
    rdfs:label "Type Specimen Designation" @en ;
    skos:inScheme :TaxonomicStatusTerms ;
    rdfs:comment "When a TNU is followed by the term `:TypeSpecimenDesignation`, the implication
  is that the specimen identified by the name in TNU should be considered a type
  of the taxon concept identified by the name as understood by the author of
  TNU."@en.

  
  :TypeSpeciesDesignation a :TaxonomicStatus ;
    rdfs:label "Type Species Designation" @en ;
    skos:inScheme :TaxonomicStatusTerms ;
    rdfs:comment "When a TNU is followed by the term `:TypeSpeciesDesignation`, the implication
  is that the taxon concept of the name in the TNU as understood by the author
  should be considered the type species of a higher taxon as understood by the
  author."@en.

  
  :NewOccurrenceRecord a :TaxonomicStatus ;
    rdfs:label "New Occurrence Record" @en ;
    skos:inScheme :TaxonomicStatusTerms ;
    rdfs:comment "When a TNU is followed by the term `:NewRecord`, the implication is that the
  description of taxon concept of the name as understood by the author is being
  extended with new occurrences (for a given locality).
  "@en.

  
  :TaxonConceptLabel a :TaxonomicStatus ;
    skos:inScheme :TaxonomicStatusTerms ;
    rdfs:label "Taxon Concept Label"@en ;
    rdfs:comment "Sometimes, incorrectly a taxon concept label (sec. Author (year) may be
  misunderstood and marked up) as a taxonomic status. This term has been created
  to indicate that a particular TNU is taxonomic concept label.
  "@en .
                


:RCC5Relation rdf:type owl:Class ;
  rdfs:subClassOf [ rdf:type owl:Restriction ;
                    owl:onProperty <http://www.w3.org/2004/02/skos/core#inScheme> ;
                    owl:someValuesFrom :RCC5RelationTerms ] ;
  rdfs:label "RCC5 Relation"@en ;
  rdfs:comment "The of RCC 5 relation, e.g. 'partially overlaps'"@en .

:RCC5RelationTerms rdf:type owl:Class ;
  rdfs:subClassOf <http://www.w3.org/2004/02/skos/core#ConceptScheme> ,
                                [ rdf:type owl:Restriction ;
                                  owl:onProperty fabio:isSchemeOf ;
                                  owl:allValuesFrom :RCC5Relation] ;
  rdfs:label "OpenBiodiv Vocabulary of RCC5 Relations"@en .

:Equals_INT rdf:type :RCC5Relation ;
  skos:inScheme :RCC5RelationTerms ;
  rdfs:label "Equals (INT)" ;
  rdfs:comment "= EQ(x,y) Equals (intensional)"@en . 

:ProperPart_INT rdf:type :RCC5Relation ;
  skos:inScheme :RCC5RelationTerms ;
  rdfs:label "Proper Part (INT)" ;
  rdfs:comment "< PP(x,y) Proper Part of (intensional)"@en .

:InverseProperPart_INT rdf:type :RCC5Relation ;
  skos:inScheme :RCC5RelationTerms ;
  rdfs:label "Inverse Proper Part (INT)" ;
  rdfs:comment "iPP(x, y) Inverse Proper Part (intensional)"@en .

:PartiallyOverlaps_INT rdf:type :RCC5Relation ;
  skos:inScheme :RCC5RelationTerms ;
  rdfs:label "Partially Overlaps (INT)" ;
  rdfs:comment "o PO(x,y) Partially Overlaps (intensional)"@en .

:Disjoint_INT rdf:type :RCC5Relation ;
  skos:inScheme :RCC5RelationTerms ;
  rdfs:label "Disjoint (INT)" ;
  rdfs:comment "! DR(x,y) Disjoint from (intensional)."@en .

:Equals_OST rdf:type :RCC5Relation ;
  skos:inScheme :RCC5RelationTerms ;
  rdfs:label "Equals (OST)" ;
  rdfs:comment "= EQ(x,y) Equals (ostensive)"@en . 

:ProperPart_OST rdf:type :RCC5Relation ;
  skos:inScheme :RCC5RelationTerms ;
  rdfs:label "Proper Part (OST)" ;
  rdfs:comment "< PP(x,y) Proper Part of (ostensive)"@en .

:InverseProperPart_OST rdf:type :RCC5Relation ;
  skos:inScheme :RCC5RelationTerms ;
  rdfs:label "Inverse Proper Part (OST)" ;
  rdfs:comment "iPP(x, y) Inverse Proper Part (ostensive)"@en .

:PartiallyOverlaps_OST rdf:type :RCC5Relation ;
  skos:inScheme :RCC5RelationTerms ;
  rdfs:label "Partially Overlaps (OST)" ;
  rdfs:comment "o PO(x,y) Partially Overlaps (ostensive)"@en .

:Disjoint_OST rdf:type :RCC5Relation ;
  skos:inScheme :RCC5RelationTerms ;
  rdfs:label "Disjoint (OST)" ;
  rdfs:comment "! DR(x,y) Disjoint from (ostensive)."@en .
