
:TaxonomicStatus rdf:type owl:Class ;
  rdfs:subClassOf [ rdf:type owl:Restriction ;
                    owl:onProperty <http://www.w3.org/2004/02/skos/core#inScheme> ;
                    owl:someValuesFrom :TaxonomicStatusTerms ] ;
  rdfs:label "Taxonomic Name Status"@en ;
  rdfs:comment "The status following a taxonomic name usage in a taxonomic
                manuscript, i.e. 'n. sp.',
                                 'comb. new',
                                 'sec. Franz (2017)', etc"@en .

:TaxonomicStatusTerms rdf:type owl:Class ;
  rdfs:subClassOf <http://www.w3.org/2004/02/skos/core#ConceptScheme> ,
                                [ rdf:type owl:Restriction ;
                                  owl:onProperty fabio:isSchemeOf ;
                                  owl:allValuesFrom :TaxonomicStatus] ;
  rdfs:label "OpenBiodiv Vocabulary of Taxonomic Name Statuses"@en ;
  fabio:hasDiscipline dbpedia:Taxonomy_(biology) .

  
  :Uncertain a :TaxonomicStatus ;
    rdfs:label "Taxonomic Uncertainty"@en ;
    rdfs:comment "This term indicates when applied to a taxonomic name
                   that there is some uncertainty about the name:
                  either in the placement of the name in the hierarchy
                  (e.g. incertae sedis), or in the description of the name
                  (e.g. nomen dubium)."@en .
  
  :New a :TaxonomicStatus ;
    rdfs:label "Taxon Discovery"@en ;
    rdfs:comment "This term when applied to a taxonomic name indicates
                  that this name denotes a taxon that is being described in
                  the present context. E.g.:
                  n. sp., gen. nov., n. trib., etc."@en .

  
  :Replacement a :TaxonomicStatus ;
    rdfs:label "Replacement Name"@en ;
    rdfs:comment "This term when applied to a taxonomic name indicates
                  that the name it is being applied to is an updated version
                  of a different name. This update may come about through
                  changes in rank (stat. n.) when the endings change (e.g.
                  -ini -> -idae), through changes in genus placement
                  (new comb.), through updates needed purely for nomenclatural
                  reasons such as to avoid homonymy or correct grammatical
                  or spelling mistakes (nomen nov.), or anything else."@en 

  :Synonym a :TaxonomicStatus .
  :Restored a :TaxonomicStatus .
  
  
  
  

