

@prefix skos: <http://www.w3.org/2004/02/skos/core#> .
@prefix pensoft: <http://id.pensoft.net/> .
@prefix rdf: <http://www.w3.org/1999/02/22-rdf-syntax-ns#> .
@prefix foaf: <http://xmlns.com/foaf/0.1/> .
@prefix pro: <http://purl.org/spar/pro/> .
@prefix scoro: <http://purl.org/spar/scoro/> .
@prefix ti: <http://www.ontologydesignpatterns.org/cp/owl/timeinterval.owl#> .
@prefix tvc: <http://www.essepuntato.it/2012/04/tvc/> .
@prefix xsd: <http://www.w3.org/2001/XMLSchema#> .
@prefix fabio: <http://purl.org/spar/fabio/> .
@prefix dcterms: <http://purl.org/dc/terms/> .
@prefix dc: <http://purl.org/dc/elements/1.1/> .
@prefix frbr: <http://purl.org/spar/frbr/> .
@prefix prism: <http://prismstandard.org/namespaces/basic/2.0> .
@prefix doco: <http://purl.org/spar/doco/> .
@prefix po: <http://www.essepuntato.it/2008/12/pattern#> .
@prefix co: <http://purl.org/co/> .
@prefix trt: <http://plazi.org/treatment#> .
@prefix c4o: <http://purl.org/spar/c4o/> .
@prefix dwciri: <http://rs.tdwg.org/dwc/iri/> .
@prefix nomen: <http://www.semanticweb.org/dmitriev/ontologies/2013/8/untitled-ontology-6#> .
@prefix dwc: <http://rs.tdwg.org/dwc/terms/> .
@prefix sro: <http://salt.semanticauthoring.org/ontologies/sro#> .
@prefix deo: <http://purl.org/spar/deo/> .
@prefix : <http://openbiodiv.net/> /

openbiodiv:
  rdf:type owl:Ontology ;
  owl:versionInfo "0.2" ;
  rdfs:comment "Open Biodiversity Knowledge Management System Core Ontology" ;
  dc:title "OpenBiodiv Core Ontology" ;
  dc:subject "OpenBiodiv Core Ontology" ;
  rdfs:label "OpenBiodiv Core Ontology" ;
  dc:creator "Viktor Senderov, Terry Catapano, Kiril Simov, Lyubomir Penev" ;
  dc:rights "CCBY" .



po:contains rdf:type owl:TransitiveProperty ;

trt:Treatment a owl:Class ;
  rdfs:label "Taxonomic Treatment"@en ;
  rdfs:label "Taxonomische Abhandlung"@de ;
  rdfs:label "Таксономично пояснение"@bg ;
  rdfs:comment "A taxonomic treatment, or simply a treatment, is a 
                rhetorical element of a taxonomic publication, i.e. a 
                specialized section, where taxon circumscription  
                takes place."@en ;
  rdfs:comment "Eine taxonomische Abhandlung, oder nur Abhandlung, ist 
                ein rhetorisches Element eines wissenschaftlichen 
                taxomischen Artikels, d.h. ein spezialisierter Abschnitt,
                wo die Umschreibung eines taxonomischen Konzeptes
                stattfindet."@de ;
  rdfs:comment "Таксономично пояснение или само Пояснение е риторчна част
                от таксономичната статия, където се случва описанието
                на дадена таксономична концепция."@bg ;                  
  rdfs:subClassOf deo:DiscourseElement .

:TaxonomicNameUsage rdf:type owl:Class ;
  rdfs:subClassOf  pext:Mention ;
  rdfs:comment "A string within a document that can be considered a mention of a
                  biological name."@en ;
  rdfs:label "Taxonomic Name Usage"@en . 

:TaxonConceptLabel rdf:type owl:Class ;
        rdfs:subClassOf :TaxonomicNameUsage ;
        rdfs:label "Taxon Concept Label"@en ;
        rdfs:comment "A taxon concept label is a taxonomic name
usage accompanied by an additional part, consisting of "sec." + an identifier
or a literature reference of a work containing the expression of a taxon concept
(treatment)." @en .



:BiologicalName rdf:type owl:Class ;
    rdfs:label "Biological Name"@en ;
    owl:sameAs nomen:NOMEN_0000030 .

:ScientificName rdf:type owl:Class ;
    rdfs:subClassOf :biologicalName ;
    rdfs:label "Scientific Name"@en ;
    owl:sameAs nomen:NOMEN_0000036 .
    
:VernacularName a owl:Class ;
  rdfs:subClassOf :biologicalName ;
  rdfs:label "Vernacular Name"@en ;
  ownl:sameAs nomen:NOMEN_0000037 .


:biologicalName rdf:type owl:ObjectProperty ;
        rdfs:label "has biological name" @en ;
        rdfs:range :BiologicalName .

:scientificName rdf:type owl:ObjectProperty ;
        rdfs:label "has scientific name" @en ;
        owl:sameAs dwciri:scientificName ;
        rdfs:range :ScientificName .

:vernacularName rdf:type owl:ObjectProperty ;
        rdfs:label "has vernacular name" @en ;
        rdfs:range :VernacularName .

:relatedName rdf:type owl:ObjectProperty, owl:TransitiveProperty, owl:ReflexiveProperty ;
  rdfs:label "has related name"@en ;
  rdfs:domain :BiologicalName ;
  rdfs:range :BiologicalName ;
  rdfs:comment "'has related name' is an object property that we
use in order to indicate that two biological names are related somehow. This
relationship is purposely vague as to encompass all situations where two
biological names co-occur in a text. It is transitive and reflexive."@en.

:replacementName rdf:type owl:ObjectProperty ,
                          owl:TransitiveProperty ,
                          owl:ReflexiveProperty ;
  rdfs:label "has replacement name"@en ;
  rdfs:domain :ScientificName ;
  rdfs:range :ScientificName ;
  rdfs:comment "This is a uni-directional property. Its meaning
is that one one biological name links to a different biological name via the
usage of this property, then the object of the triple is the form of the
biological name the use of which is more accurate and should be preferred
given the information that system currently holds. This property is only
defined for scientific names."@en.


:TaxonConcept rdf:type owl:Class ;
  owl:sameAs dwc:Taxon ;
  rdfs:subClassof frbr:Work ,
                  skos:Concept ,
                  [ rdf:type owl:Restriction ;
                    owl:onProperty frbr:realization ;
                    owl:minCardinality "1" ] ,
                  [ rdf:type owl:Restriction ;
                    owl:onProperty :biologicalName ;
                    owl:minCardinality "1" ] .


@prefix : <http://openbiodiv.net/> .
@prefix skos: <http://www.w3.org/2004/02/skos/core#> .

:TaxonomicStatus rdf:type owl:Class ;
  rdfs:subClassOf [ rdf:type owl:Restriction ;
                    owl:onProperty <http://www.w3.org/2004/02/skos/core#inScheme> ;
                    owl:someValuesFrom :TaxonomicStatusTerms ] ;
  rdfs:label "Taxonomic Status"@en ;
  rdfs:comment "The status following a taxonomic name usage in a taxonomic
                manuscript, i.e. 'n. sp.',
                                 'comb. new',
                                 'sec. Franz (2017)', etc"@en .

:TaxonomicStatusTerms rdf:type owl:Class ;
  rdfs:subClassOf <http://www.w3.org/2004/02/skos/core#ConceptScheme> ,
                                [ rdf:type owl:Restriction ;
                                  owl:onProperty fabio:isSchemeOf ;
                                  owl:allValuesFrom :TaxonomicStatus] ;
  rdfs:label "OpenBiodiv Vocabulary of Taxonomic Statuses"@en ;
  fabio:hasDiscipline dbpedia:Taxonomy_(biology) .

  
  :TaxonomicUncertainty a :TaxonomicStatus ;
    rdfs:label "Taxonomic Uncertainty"@en ;
    skos:inScheme :TaxonomicStatusTerms ;
    skos:related <http://rs.gbif.org/vocabulary/gbif/taxonomicStatus/accepted> ;
   
    rdfs:comment "The implication of this term that the taxon concept identified
  by a name has an uncertain placement in the biological taxonomy, or if we
  are talking about a specimen or a sample of some kind that we are unable to
  identify the taxon down to its rank. "@en .

  
  :TaxonDiscovery a :TaxonomicStatus ;
    skos:inScheme :TaxonomicStatusTerms ;
    rdfs:label "Taxon Discovery"@en ;

    rdfs:comment "When a TNU is followed by the term `:TaxonDiscovery`, the
  implication is that the present context in which the TNU is used is
  circumscribing a new taxon concept (a taxon concept of a taxon new to
  science), and simultaneously assigning it a new name."@en .

  
  :ReplacementName a :TaxonomicStatus ;
    skos:inScheme :TaxonomicStatusTerms ;
    rdfs:label "Replacement Name"@en ;
    rdfs:comment "When a TNU is followed by the term `:ReplacementName`, the implication is that
  the name that is referred to by the TNU is replacing another name for various
  reasons, and thus becoming the preferred/accepted/available way of refering to
  whatever taxon concepts the now replaced name had been referring to. Cases
  include changes of rank, new combinations, spelling mistakes, etc.
  "@en .

  
  :UnavailabeName a :TaxonomicStatus ;
    skos:inScheme :TaxonomicStatusTerms ;
    rdfs:label "UnavailableName"@en ;
    skos:exactMatch  <http://rs.gbif.org/vocabulary/gbif/taxonomicStatus/synonym> ;
    rdfs:comment "When a TNU is followed by the term `:UnavailableName`, the implication is that
  the name that is being referred to by the TNU is no longer or has never been
  available for use due to the fact that it has either been replaced or it has
  been determined that the name has been improperly coined or published, or the
  name contains any general error rendering it unfit for use."@en .


  <<Available Name>
  
  :TypeSpecimenDesignation a :TaxonomicStatus ;
    rdfs:label "Type Specimen Designation" @en ;
    skos:inScheme :TaxonomicStatusTerms ;
    rdfs:comment "When a TNU is followed by the term `:TypeSpecimenDesignation`, the implication
  is that the specimen identified by the name in TNU should be considered a type
  of the taxon concept identified by the name as understood by the author of
  TNU."@en.

  
  :TypeSpeciesDesignation a :TaxonomicStatus ;
    rdfs:label "Type Species Designation" @en ;
    skos:inScheme :TaxonomicStatusTerms ;
    rdfs:comment "When a TNU is followed by the term `:TypeSpeciesDesignation`, the implication
  is that the taxon concept of the name in the TNU as understood by the author
  should be considered the type species of a higher taxon as understood by the
  author."@en.

  
  :NewOccurrenceRecord a :TaxonomicStatus ;
    rdfs:label "New Occurrence Record" @en ;
    skos:inScheme :TaxonomicStatusTerms ;
    rdfs:comment "When a TNU is followed by the term `:NewRecord`, the implication is that the
  description of taxon concept of the name as understood by the author is being
  extended with new occurrences (for a given locality).
  "@en.

  
  :TaxonConceptLabel a :TaxonomicStatus ;
    skos:inScheme :TaxonomicStatusTerms ;
    rdfs:label "Taxon Concept Label"@en ;
    rdfs:comment "Sometimes, incorrectly a taxon concept label (sec. Author (year) may be
  misunderstood and marked up) as a taxonomic status. This term has been created
  to indicate that a particular TNU is taxonomic concept label.
  "@en .
                



  # Parts of PROTON

top:Entity rdf:type owl:Class ;
            rdfs:comment "Any sort of an entity of interest, usually something existing, happening, or purely abstract. Entities may have several - more than one - names or aliases."@en ;
            rdfs:label "Entity"@en .

ptop:Object rdf:type owl:Class ;
            rdfs:subClassOf ptop:Entity ;
            rdfs:comment "Objects are entities that could be claimed to exist - in some sense of existence. An object can play a certain role in some happenings. Objects could be substantially real - as the Buckingham Palace or a hardcopy book - or substantially imperceptible - for instance, an electronic document that exists only virtually, one cannot touch it."@en ;
            rdfs:label "Object"@en .

ptop:Statement rdf:type owl:Class ;
               rdfs:subClassOf ptop:Object ;
               rdfs:comment "A message that is stated or declared; a communication (oral or written), setting forth particulars or facts, etc; \"according to his statement he was in London on that day\". WordNet 1.7.1"@en ;
               rdfs:label "Statement"@en .

ptop:InformationResource rdf:type owl:Class ;
                         rdfs:subClassOf ptop:Statement ;
                         rdfs:comment "InformationResource denotes an information resource with identity, as defined in Dublin Core (DC2003ISO). InformationResource is considered any communication or message that is delivered or produced, taking into account the specific intention of its originator, and also the supposition (and anticipation) for a particular audience or counter-agent in the process of communication (i.e. passive or active feed-back)."@en ;
                         rdfs:label "Information Resource"@en .

pkm:mentions
      rdf:type owl:ObjectProperty ;
      rdfs:comment """
    A direct link between an information resource, like a document or a section and an entity.
  """ ;
      rdfs:domain ptop:InformationResource ;
      rdfs:label "mentions" ;
      rdfs:range psys:Entity .

pext:Mention rdf:type owl:Class ;
             rdfs:subClassOf ptop:InformationResource ;
             rdfs:comment "An area of a document that can be considered a mention of something."@en ;
             rdfs:label "Section" .
